src/UInt256.ec
@@ -1,17 +1,52 @@
 pragma Goals:printall.
 
+require import AllCore.
 require export Int IntDiv JWord.
 
+type uint8 = W8.t. (*specifically used for storing bytes in the memory map*)
 type uint256 = W256.t.
 
 abbrev (%%) (m d : uint256) = W256.\umod m d.
 abbrev (<)  (a b : uint256) = W256.\ult a b.
 abbrev (<=) (a b : uint256) = W256.\ule a b.
 
+op uint256_as_signed (x : uint256) : int =
+  if W256.to_uint x < 340282366920938463463374607431768211456
+  then W256.to_uint x
+  else - (340282366920938463463374607431768211457 - (W256.to_uint x)).
 op bool_of_uint256 (x : uint256) : bool = x <> W256.zero.
-op eq_uint256(a : uint256, b : uint256) : uint256  = if a = b then W256.one else W256.zero.
+
+(* op try_u256_to_u8 (x: uint256) : uint8 option =
+  if W256.to_uint x < (2^8)
+  then Some (W8.of_int (W256.to_uint x))
+  else None. *)
 
 lemma neg_w256_zero_eq_w256_zero : - W256.zero = W256.zero.
     proof.
-      smt.
+      smt (@W256).
+  qed.
+
+lemma eq_sub_of_add_eq (x y z : uint256) : x + y = z => x = z - y.
+  proof.
+    progress.
+    smt (@W256).
+  qed.
+
+lemma neq_sub_of_add_neq (x y z : uint256) : x + y <> z => x <> z - y.
+  proof.
+    progress.
+    smt (@W256).
+  qed.
+
+lemma lt_or_eq_of_lt_succ (a l : uint256) : a < l + W256.one => a < l \/ a = l.
+  proof.
+    case (a < l).
+    progress.
+    progress.
+    admit.
+  qed.
+
+lemma zero_of_to_uint_zero (x: uint256): to_uint x = 0 => x = W256.zero.
+    proof.
+      by smt(@W256).
   qed.
