src/YulTests.ec
@@ -1,0 +1,421 @@
+pragma Goals:printall.
+
+require import AllCore.
+require import Array.
+require import ExtractedTests.
+require import Int.
+require import IntDiv.
+require import Memory.
+require import Real.
+require import UInt256.
+require import YulPrimops.
+require import PurePrimops.
+require import Utils.
+require import JUtils.
+
+import MemoryMap.
+
+lemma is_even_correcteness (x: uint256) :
+hoare [ YulTest.is_even : arg = x ==> (
+    x %% W256.of_int 2 = W256.zero => res = W256.one
+      ) /\ (x %% W256.of_int 2 <> W256.zero => res = W256.zero) ].
+    proof.
+      proc.
+      wp. skip. progress. smt.
+      smt.
+    qed.
+  
+lemma writeReadTest_correctness :
+
+    forall (address value: uint256),
+phoare [ YulTest.writeReadTest :
+      arg = (address, value) ==>
+      res = value] = 1%r.
+proof.
+    progress.
+  proc.
+  exists* Primops.memory.
+  elim*=>memory_pre.
+  wp.
+  call (ConcretePrimops.mload_pspec (PurePrimops.mstore memory_pre address value) address).
+  call (ConcretePrimops.mstore_pspec memory_pre address value).
+  skip.
+  progress.
+  apply load_store_same.
+qed.
+  
+lemma revert_if_two_correctness (x : uint256) :
+    phoare [YulTest.revert_if_two : arg = x /\ !Primops.reverted ==>
+      (res = x + (W256.of_int 3)/\ x <> (W256.of_int 2) /\ !Primops.reverted) \/ (x = (W256.of_int 2) /\ Primops.reverted)] = 1%r.
+        proc.
+        inline Primops.revert.
+        wp.
+        skip.
+        progress.
+        rewrite /bool_of_uint256 /eq_uint256 in H0.
+        have H1 : x{hr} + (of_int 3)%W256 = (of_int 5)%W256. smt ().
+        rewrite (eq_sub_of_add_eq _ _ _ H1).
+        progress.
+        left.
+        rewrite /bool_of_uint256 /eq_uint256 in H0.
+        have H1 : x{hr} + (of_int 3)%W256 <> (of_int 5)%W256. smt (@W256).
+        have H2 := neq_sub_of_add_neq _ _ _ H1.
+        progress.
+  qed.
+
+lemma shifty_correctness (x s : uint256) :
+    phoare [YulTest.shifty : arg = (x, s) /\ !Primops.reverted ==>
+      (res = x /\ !Primops.reverted) \/ ((W256.of_int 256) < s /\ Primops.reverted)] = 1%r.
+        proc.
+        case ((W256.of_int 256) < s).
+        rcondt 1.
+        skip. progress.
+        rewrite /bool_of_uint256 /gt_uint256. by smt (@W256).
+        inline Primops.revert.
+        wp.
+        skip.
+        by progress.
+        rcondf 1.
+        skip. progress.
+        rewrite /bool_of_uint256 /gt_uint256. by smt (@W256).
+        wp. skip. progress. 
+        left.
+        split; first last.
+        exact H.
+        rewrite /shr /shl.
+        pose sh := to_uint s{hr}.
+        pose sh' := to_uint ((W256.of_int 256) - s{hr}).
+        rewrite W256.shrl_andmaskN. smt (@W256).
+    case (to_uint s{hr} = 256).
+        progress.
+        rewrite /sh H1.
+        pose v := x{hr}.
+        have H2 : v `<<<` 256 = W256.zero. smt (@W256).
+        have H3 : forall (s : int), W256.zero `>>>` s = W256.zero. progress. smt (@W256).
+        have H4 : sh' = 0. smt (@W256).
+        rewrite H2 H3 H4. simplify.
+        smt (@W256).
+        progress.
+        rewrite W256.shlw_shrw_shlw. rewrite /sh.
+        have H5 := (W256.to_uint_cmp s{hr}).
+        simplify. progress.
+        smt ().
+        smt (@W256).
+        simplify.
+        rewrite shl_zero.
+        have H6 : sh' = 256 - sh. smt.
+        rewrite -H6.
+        have H7 : x{hr} `&` (W256.masklsb sh') = (splitMask (W256.masklsb sh') x{hr}).`1. smt ().
+        have H8 : x{hr} `&` (W256.invw (W256.masklsb sh')) = (splitMask (W256.masklsb sh') x{hr}).`2. smt ().
+        rewrite H7 H8.
+        exact W256.splitMask_add.
+  qed.  
+  
+lemma mod_test_correctness (m : uint256) :
+    phoare [YulTest.mod_test : arg = m /\ W256.one < m ==> res = W256.zero] = 1%r.
+    proc.
+    wp.
+    skip.
+    rewrite /PurePrimops.mulmod /PurePrimops.addmod.
+    progress.
+    have H0 : to_uint (m{hr} - W256.one) = (to_uint m{hr}) - 1. rewrite W256.to_uintB. smt (@W256). smt (@W256).
+    rewrite H0.
+    pose modu := to_uint m{hr}.
+    have H1 : (modu - 1) * (modu - 1) = modu * (modu - 2) + 1. smt ().
+    have H2 : (modu * (modu - 2) + 1) %% modu = 1. rewrite mul_add_mod_eq /modu. smt (@W256). smt (@W256).
+    rewrite H1 H2.
+    simplify.
+    smt (@W256).
+  qed.
+  
+lemma keccak_correctness (addr1 addr2 sz : uint256) : equiv [Primops.keccak256 ~ Primops.keccak256 : arg{1} = (addr1, sz) /\ arg{2} = (addr2, sz) /\ forall (i : uint256), W256.zero <= i /\ i < sz => Primops.memory{1}.[addr1 + i] = Primops.memory{2}.[addr2 + i] ==> res{1} = res{2}].
+    proc.
+    wp. skip.
+    progress.
+    congr.
+    apply eq_from_get.
+    smt (@Array).
+    rewrite Array.size_offun.
+    progress.
+    have H_i: i < to_uint size{1} by smt(@W256).
+    rewrite Array.offunE. smt ().
+    rewrite Array.offunE. smt ().
+    progress.
+    apply H.
+    smt (@W256).
+  qed.
+
+lemma splitMask_zero mask: W256.splitMask mask W256.zero = (W256.zero, W256.zero).
+    proof.
+      by smt(@W256).
+  qed.
+
+lemma zero_shl s: W256.zero `<<<` s = W256.zero.
+    proof.
+      by smt(@W256).
+    qed.
+
+lemma zero_shr s: W256.zero `>>>` s = W256.zero.
+    proof.
+      by smt(@W256).
+    qed.
+
+    hint simplify splitMask_zero, zero_shl, zero_shr.
+
+lemma mstore8_test_correctness (a b: uint256): hoare[
+    YulTest.mstore8test :
+      arg = (a,b) /\ a < W256.of_int 256 /\ b < W256.of_int 256 ==> res = ((a `<<<` 8) `|` b) `<<<` 240
+    ].
+    proof.
+      proc.
+
+      inline *.
+      wp.
+      skip.
+      progress.
+      rewrite loadE storeE.
+      simplify.
+      do 32! rewrite W32u8.get_zero.
+      apply W256.ext_eq.
+      progress.
+      rewrite W32u8.pack32wE. smt ().
+      have H_256: 0 <= x0 && x0 < 256 by smt ().
+      rewrite H_256. progress.
+      pose byte_idx := x0 %/ 8.
+      pose bit_idx := x0 %% 8.
+    case (x0 < 240).
+      progress.
+      have H_lhs: !(0 <= x0 - 240 && x0 - 240 < 256) by smt ().
+      rewrite H_lhs. progress.
+      have H_byte_idx_low: 0 <= byte_idx by smt ().
+      have H_byte_idx_high: byte_idx < 30 by smt ().
+      rewrite W32u8.Pack.initE.
+      have H_byte_idx_wide_range: 0 <= byte_idx && byte_idx < 32 by smt ().
+      rewrite H_byte_idx_wide_range.
+      progress. 
+      pose idx' := 31 - byte_idx.
+      have H_idx'_low: 2 <= idx' by smt ().
+      have H_idx'_high: idx' < 32 by smt ().
+      rewrite Map.get_set_neqE. smt.
+      rewrite Map.get_set_neqE. smt.
+      have H_y : y{hr}.[x0-240] = false by smt (@W256).
+      rewrite H_y.
+    search W8."_.[_]".
+      rewrite - (W8.zerowE (bit_idx)).
+      congr.
+      have H_diff: forall (i j: int), 0 <= i < 32 => 0 <= j < 32 => i <> j => W256.of_int i <> W256.of_int j.
+      progress.
+      smt.
+      smt (Map.get_set_sameE Map.get_set_neqE).
+      progress.
+      rewrite W32u8.Pack.initE.
+    case (byte_idx = 30). progress.
+      rewrite H4.
+      progress.
+      have H_x0: 240 <= x0 < 248 by smt ().
+      have H_x0_range: (0 <= x0 - 240 && x0 - 240 < 256) by smt ().
+      rewrite H_x0_range. progress.
+    search W256."_.[_]".
+      rewrite W256.get_out. smt ().
+      rewrite Map.get_set_sameE.
+      have H_lhs: 0 <= x0 && x0 < 256 by smt().
+      simplify.
+      have H_bit_idx: bit_idx = x0-240 by smt().
+      rewrite - H_bit_idx.
+      smt.
+    case (byte_idx = 31). progress.
+      rewrite H4.
+      progress.
+      have H_x0: 248 <= x0 < 256 by smt().
+      have H_small: forall (a: uint256) (b: int), a < W256.of_int 256 => 8 <= b => a.[b] = false.
+      progress.
+    search W256."_.[_]".
+      pose a8 := W8.of_int (W256.to_uint a).
+      have H_a8: forall (i: int), a.[i] = a8.[i] by smt.
+      rewrite H_a8. smt.
+      rewrite (H_small (y{hr})). assumption. smt (). simplify.
+      have H_lhs: (0 <= x0 - 240 && x0 - 240 < 256) by smt().
+      rewrite H_lhs. simplify.
+      rewrite Map.get_set_neqE. smt (@W256).
+      rewrite (Map.get_set_sameE _ W256.zero).
+      have H_bit_idx: bit_idx = x0 - 248 by smt ().
+      rewrite -H_bit_idx.
+      smt.
+      smt ().
+    qed.
+
+lemma modexp_test_correctness (a b c: uint256): hoare [ YulTest.modexp_test: arg = (a, b, c) ==> res = (W256.one, (
+    W256.of_int (
+            ((W256.to_uint a) ^ (W256.to_uint b)) %% (W256.to_uint c)
+    )
+  ))].
+      proc.
+      exists* Primops.memory.
+      elim*. progress.
+      pose mem_1 := PurePrimops.mstore memory W256.zero (W256.of_int 32).
+      pose mem_2 := PurePrimops.mstore mem_1 (W256.of_int 32) (W256.of_int 32).
+      pose mem_3 := PurePrimops.mstore mem_2 (W256.of_int 64) (W256.of_int 32).
+      pose mem_4 := PurePrimops.mstore mem_3 (W256.of_int 96) a.
+      pose mem_5 := PurePrimops.mstore mem_4 (W256.of_int 128) b.
+      pose mem_6 := PurePrimops.mstore mem_5 (W256.of_int 160) c.
+      have H_mem6_get0: PurePrimops.mload mem_6 W256.zero = W256.of_int 32.
+      do 5! ((rewrite load_store_diff; first smt(@W256)); first smt(@W256)).
+      rewrite load_store_same. reflexivity.
+      have H_mem6_get32: PurePrimops.mload mem_6 (W256.of_int 32) = W256.of_int 32.
+      do 4! ((rewrite load_store_diff; first smt(@W256)); first smt(@W256)).
+      rewrite load_store_same. reflexivity.
+      have H_mem6_get64: PurePrimops.mload mem_6 (W256.of_int 64) = W256.of_int 32.
+      do 3! ((rewrite load_store_diff; first smt(@W256)); first smt(@W256)).
+      rewrite load_store_same. reflexivity.
+      have H_mem6_get96: PurePrimops.mload mem_6 (W256.of_int 96) = a.
+      do 2! ((rewrite load_store_diff; first smt(@W256)); first smt(@W256)).
+      rewrite load_store_same. reflexivity.
+      have H_mem6_get128: PurePrimops.mload mem_6 (W256.of_int 128) = b.
+      rewrite load_store_diff. smt(@W256). smt(@W256).
+      rewrite load_store_same. reflexivity.
+      have H_mem6_get160: PurePrimops.mload mem_6 (W256.of_int 160) = c.
+      rewrite load_store_same. reflexivity.
+      seq 6 : (Primops.memory = mem_6 /\ x = a /\ y = b /\ z = c).
+      call (ConcretePrimops.mstore_spec mem_5 (W256.of_int 160) c).
+      call (ConcretePrimops.mstore_spec mem_4 (W256.of_int 128) b).
+      call (ConcretePrimops.mstore_spec mem_3 (W256.of_int 96) a).
+      call (ConcretePrimops.mstore_spec mem_2 (W256.of_int 64) (W256.of_int 32)).
+      call (ConcretePrimops.mstore_spec mem_1 (W256.of_int 32) (W256.of_int 32)).
+      call (ConcretePrimops.mstore_spec memory W256.zero (W256.of_int 32)).
+      skip. by progress.
+      inline Primops.staticcall.
+      sp.
+      rcondt 1. skip. by progress.
+      rcondt 4.
+      call (ConcretePrimops.mload_spec mem_6 (W256.of_int 64)).
+      call (ConcretePrimops.mload_spec mem_6 (W256.of_int 32)).
+      call (ConcretePrimops.mload_spec mem_6 W256.zero).
+      skip. progress.
+      seq 6: (
+        #pre /\
+        bsize = W256.of_int 32 /\
+        esize = W256.of_int 32 /\
+        msize = W256.of_int 32 /\
+        base = a /\
+        exp = b /\
+        mod = c
+      ).
+      call (ConcretePrimops.mload_spec mem_6 (W256.of_int 160)).
+      call (ConcretePrimops.mload_spec mem_6 (W256.of_int 128)).
+      call (ConcretePrimops.mload_spec mem_6 (W256.of_int 96)).
+      call (ConcretePrimops.mload_spec mem_6 (W256.of_int 64)).
+      call (ConcretePrimops.mload_spec mem_6 (W256.of_int 32)).
+      call (ConcretePrimops.mload_spec mem_6 W256.zero).
+          skip. progress.
+          pose result := (W256.of_int ((W256.to_uint a) ^ (W256.to_uint b) %% (W256.to_uint c))).
+          pose mem_7 := PurePrimops.mstore mem_6 W256.zero result.
+          wp.
+          call (ConcretePrimops.mload_spec mem_7 W256.zero).
+          wp.
+          call (ConcretePrimops.mstore_spec mem_6 W256.zero result).
+          skip. progress.
+          rewrite /mem_7.
+          rewrite load_store_same.
+          reflexivity.
+      qed.
+
+
+      
+lemma calldata_test_correctness (ind : uint256) :
+    phoare [YulTest.calldata_test : arg = ind ==> res = W256.one] = 1%r.
+    proc.
+    inline Primops.calldataload.
+    wp.
+    skip.
+    progress.
+    smt ().
+  qed.
+
+lemma aux_range (x: int): 0<=x<32 => !(W256.of_int 64 <= W256.of_int (31 - x)).
+    proof.
+      progress.
+      smt.
+    qed.
+  
+      lemma aux_range2 (x: int): 0<=x<32 => !(W256.of_int 64 <= W256.of_int (63 - x)).
+        proof.
+          progress.
+          smt.
+        qed.
+
+lemma ret_test_correctness (a b: uint256) :
+    phoare [
+      YulTest.ret_test :
+      arg = (a,b) ==>
+      load Primops.ret_data W256.zero = a /\
+      load Primops.ret_data (W256.of_int 32) = b
+    ] = 1%r.
+    proof.
+      proc.
+      exists* Primops.memory.
+      elim*.
+      progress.
+      inline *. wp.
+      skip.
+      progress.
+      rewrite /load.
+      apply W256.ext_eq.
+      progress.
+    print pack32wE.
+      rewrite pack32wE. by trivial.
+      rewrite W32u8.Pack.initE.
+      have H_in_range: 0 <= x %/ 8 && x %/ 8 < 32 by smt ().
+      rewrite H_in_range. progress.
+      rewrite Map.offunE. progress.
+      have H_in_range2: !(W256.of_int 64 <= W256.of_int (31 - x %/ 8)).
+      apply (aux_range (x %/ 8)). by trivial.
+      rewrite H_in_range2. progress.
+      rewrite /store. progress.
+      have H_diff: forall (i j: int), 0<=i<32 => 32<=j<64 => W256.of_int i <> W256.of_int j.
+      progress. smt.
+      pose byte_idx:= 31 - x %/ 8.
+      have H_byte_idx: 0<=byte_idx<32 by smt ().
+      do 32! (rewrite Map.get_set_neqE; first exact H_diff).
+      have H_a: (load (store Primops.memory{hr} W256.zero a{hr}) W256.zero).[x] = a{hr}.[x] by smt (load_store_same).
+      rewrite- H_a.
+      rewrite /byte_idx.
+      rewrite /load /store.
+      rewrite pack32wE. by trivial.
+      rewrite W32u8.Pack.initE.
+      rewrite H_in_range. simplify. by trivial.
+      pose mem_1:= store Primops.memory{hr} W256.zero a{hr}.
+      have H_b: load (store mem_1 (W256.of_int 32) b{hr}) (W256.of_int 32) = b{hr} by exact load_store_same.
+      rewrite -H_b.
+      rewrite /load.
+      pose mem := store mem_1 (W256.of_int 32) b{hr}.
+      have H_inner: forall (i: int), 0<=i<32 =>
+        ((Map.offun (fun (i0: uint256) => (
+          if W256.of_int 64 <= i0
+          then witness
+          else (store mem_1 (W256.of_int 32) (pack32_t (W32u8.Pack.init (fun (i1: int) => mem.[W256.of_int (63-i1)])))).[i0]
+            ))).[W256.of_int (63-i)] = mem.[W256.of_int (63-i)]).
+                progress.
+                rewrite Map.offunE. progress.
+                have H_if: !(W256.of_int 64 <= W256.of_int (63-i)). smt.
+                rewrite H_if. progress.
+                rewrite /mem /store. progress.
+                smt.
+                apply W256.ext_eq. progress.
+                rewrite pack32wE. trivial.
+                rewrite initE.
+                have H_range: 0 <= x %/ 8 && x %/ 8 < 32 by smt ().
+                rewrite H_range. progress.
+                rewrite Map.offunE. progress.
+                have H_range': !(W256.of_int 64 <= W256.of_int (63 - x %/ 8)) by exact aux_range2.
+                rewrite H_range'. progress.
+                rewrite /store. progress.
+                rewrite pack32wE. by trivial.
+                rewrite initE.
+                rewrite H_range. progress.
+                congr.
+                pose idx := x %/ 8.
+                have H_diff: forall (i j: int), 32<=i<64 => 32<=j<64 => i <> j => W256.of_int i <> W256.of_int j.
+                progress. smt.
+                smt (Map.get_set_sameE Map.get_set_neqE).
+      qed.      
+
